Hashmap/DHashMap/Model.lean
@@ -4,6 +4,7 @@ Released under Apache 2.0 license as described in the file LICENSE.
 Authors: Markus Himmel
 -/
 import Hashmap.DHashMap.Basic
+import Hashmap.DHashMap.ForUpstream
 
 /-!
 In this file we define functions for manipulating a hash map based on operations defined in terms of their buckets.
@@ -20,6 +21,8 @@ variable {α : Type v} {β : α → Type v}
 
 namespace MyLean.DHashMap
 
+/-! # Setting up the infrastructure -/
+
 def bucket [Hashable α] (self : Array (AssocList α β)) (h : 0 < self.size) (k : α) : AssocList α β :=
   let ⟨i, h⟩ := mkIdx (hash k) h
   self[i]
@@ -34,7 +37,70 @@ theorem size_updateBucket [Hashable α] {self : Array (AssocList α β)} {h : 0 
     {f : AssocList α β → AssocList α β} : (updateBucket self h k f).size = self.size := by
   simp [updateBucket]
 
+open List
+
+theorem exists_bucket_of_uset [BEq α] [Hashable α]
+  (self : Array (AssocList α β)) (i : USize) (hi : i.toNat < self.size) (d : AssocList α β) :
+    ∃ l, toListModel self ~ self[i.toNat].toList ++ l ∧
+      toListModel (self.uset i d hi) ~ d.toList ++ l ∧
+      (∀ [EquivBEq α] [LawfulHashable α],
+        IsHashSelf self → ∀ k : α, (mkIdx (hash k) (show 0 < self.size by omega)).1.toNat = i.toNat → l.containsKey k = false) := by
+  have h₀ : 0 < self.size := by omega
+  obtain ⟨l₁, l₂, h₁, h₂, h₃⟩ := Array.exists_of_update self i d hi
+  refine ⟨l₁.bind AssocList.toList ++ l₂.bind AssocList.toList, ?_, ?_, ?_⟩
+  · rw [toListModel, h₁]
+    simpa using List.perm_append_comm_assoc _ _ _
+  · rw [toListModel, h₃]
+    simpa using List.perm_append_comm_assoc _ _ _
+  · intro _ _ h k
+    rw [← Decidable.not_imp_not]
+    intro hk
+    simp only [Bool.not_eq_false, containsKey_eq_true_iff_exists_mem, mem_append, mem_bind] at hk
+    obtain ⟨⟨k', v'⟩, ⟨(⟨a, ha₁, ha₂⟩|⟨a, ha₁, ha₂⟩), hk⟩⟩ := hk
+    · obtain ⟨n, hn⟩ := List.get_of_mem ha₁
+      rw [List.get_eq_get_append_right (self[i] :: l₂)] at hn
+      suffices (mkIdx (hash k') h₀).1.toNat = n from
+        Nat.ne_of_lt (Nat.lt_of_eq_of_lt (hash_eq hk ▸ this) (h₂ ▸ n.2))
+      rw [List.get_congr h₁.symm, ← Array.getElem_eq_data_get] at hn
+      exact (h.hashes_to n (by omega)).hash_self h₀ _ (hn.symm ▸ ha₂)
+    · obtain ⟨n, hn⟩ := List.get_of_mem ha₁
+      rw [List.get_eq_get_cons self[i], List.get_eq_get_append_left l₁] at hn
+      suffices (mkIdx (hash k') h₀).1.toNat = n + 1 + l₁.length by
+        refine Nat.ne_of_lt' ?_
+        simp only [← hash_eq hk, this, h₂, Nat.lt_add_left_iff_pos, Nat.succ_pos]
+      rw [List.get_congr h₁.symm, ← Array.getElem_eq_data_get] at hn
+      refine (h.hashes_to (n + 1 + l₁.length) ?_).hash_self h₀ _ (hn.symm ▸ ha₂)
+      rw [Array.size_eq_length_data, h₁, length_append, length_cons]
+      omega
+
+theorem exists_bucket_of_update [BEq α] [Hashable α] (m : Array (AssocList α β)) (h : 0 < m.size) (k : α)
+    (f : AssocList α β → AssocList α β) :
+    ∃ l : List (Σ a, β a),
+      toListModel m ~ (bucket m h k).toList ++ l ∧
+      toListModel (updateBucket m h k f) ~ (f (bucket m h k)).toList ++ l ∧
+      (∀ [EquivBEq α] [LawfulHashable α], IsHashSelf m → ∀ k', hash k = hash k' → l.containsKey k' = false) := by
+  let idx := mkIdx (hash k) h
+  obtain ⟨l, h₁, h₂, h₃⟩ := exists_bucket_of_uset m idx.1 idx.2 (f m[idx.1])
+  exact ⟨l, h₁, h₂, fun h k' hk' => h₃ h _ (hk' ▸ rfl)⟩
+
+theorem exists_bucket' [BEq α] [Hashable α]
+    (self : Array (AssocList α β)) (i : USize) (hi : i.toNat < self.size) :
+      ∃ l, self.data.bind AssocList.toList ~ self[i.toNat].toList ++ l ∧
+        (∀ [EquivBEq α] [LawfulHashable α], IsHashSelf self → ∀ k,
+          (mkIdx (hash k) (show 0 < self.size by omega)).1.toNat = i.toNat → l.containsKey k = false) := by
+  obtain ⟨l, h₁, -, h₂⟩ := exists_bucket_of_uset self i hi .nil
+  exact ⟨l, h₁, h₂⟩
+
+theorem exists_bucket [BEq α] [Hashable α]
+    (m : Array (AssocList α β)) (h : 0 < m.size) (k : α) :
+    ∃ l : List (Σ a, β a), toListModel m ~ (bucket m h k).toList ++ l ∧
+      (∀ [EquivBEq α] [LawfulHashable α], IsHashSelf m → ∀ k', hash k = hash k' → l.containsKey k' = false) := by
+  obtain ⟨l, h₁, -, h₂⟩ := exists_bucket_of_update m h k (fun _ => .nil)
+  exact ⟨l, h₁, h₂⟩
+
 namespace Raw₀
+
+/-! # Definition of model functions -/
 
 def replaceₘ [BEq α] [Hashable α] (m : Raw₀ α β) (a : α) (b : β a) : Raw₀ α β :=
   ⟨⟨m.1.size, updateBucket m.1.buckets m.2 a (fun l => l.replace a b)⟩, by simpa using m.2⟩
@@ -42,26 +108,32 @@ def replaceₘ [BEq α] [Hashable α] (m : Raw₀ α β) (a : α) (b : β a) : R
 def consₘ [BEq α] [Hashable α] (m : Raw₀ α β) (a : α) (b : β a) : Raw₀ α β :=
   ⟨⟨m.1.size + 1, updateBucket m.1.buckets m.2 a (fun l => l.cons a b)⟩, by simpa using m.2⟩
 
-def insertₘ [BEq α] [Hashable α] (m : Raw₀ α β) (a : α) (b : β a) : Raw₀ α β :=
-  if (bucket m.1.buckets m.2 a).contains a then replaceₘ m a b else Raw₀.expandIfNecessary (consₘ m a b)
-
 def findEntry?ₘ [BEq α] [Hashable α] (m : Raw₀ α β) (a : α) : Option (Σ a, β a) :=
   (bucket m.1.buckets m.2 a).findEntry? a
+
+def containsₘ [BEq α] [Hashable α] (m : Raw₀ α β) (a : α) : Bool :=
+  (bucket m.1.buckets m.2 a).contains a
+
+def insertₘ [BEq α] [Hashable α] (m : Raw₀ α β) (a : α) (b : β a) : Raw₀ α β :=
+  if m.containsₘ a then m.replaceₘ a b else Raw₀.expandIfNecessary (m.consₘ a b)
+
+/-! # Equivalence between model functions and real implementations -/
 
 theorem reinsertAux_eq [Hashable α] (data : { d : Array (AssocList α β) // 0 < d.size }) (a : α) (b : β a) :
     (reinsertAux data a b).1 = updateBucket data.1 data.2 a (fun l => l.cons a b) := rfl
 
-theorem insert_eq_insertₘ [BEq α] [Hashable α] (m : Raw₀ α β) (a : α) (b : β a) :
-    (insert m a b).1 = insertₘ m a b := by
-  rw [insert, insertₘ, bucket]
-  apply Subtype.eq
-  dsimp
-  split
-  · rfl
-  · rfl
-
 theorem findEntry?_eq_findEntry?ₘ [BEq α] [Hashable α] (m : Raw₀ α β) (a : α) :
     findEntry? m a = findEntry?ₘ m a := rfl
+
+theorem contains_eq_containsₘ [BEq α] [Hashable α] (m : Raw₀ α β) (a : α) :
+    m.contains a = m.containsₘ a := rfl
+
+theorem insert_eq_insertₘ [BEq α] [Hashable α] (m : Raw₀ α β) (a : α) (b : β a) :
+    (insert m a b).1 = insertₘ m a b := by
+  rw [insert, insertₘ, containsₘ, bucket]
+  apply Subtype.eq
+  dsimp only [Array.ugetElem_eq_getElem, Array.uset]
+  split <;> rfl
 
 end Raw₀
 
